@prefix dbo: <http://dbpedia.org/ontology/> .
@prefix owl: <http://www.w3.org/2002/07/owl#> .
@prefix rdf: <http://www.w3.org/1999/02/22-rdf-syntax-ns#> .
@prefix xml: <http://www.w3.org/XML/1998/namespace> .
@prefix xsd: <http://www.w3.org/2001/XMLSchema#> .
@prefix foaf: <http://xmlns.com/foaf/spec/#> .
@prefix rdfs: <http://www.w3.org/2000/01/rdf-schema#> .
@prefix skos: <http://www.w3.org/2004/02/skos/core#> .
@prefix void: <http://rdfs.org/ns/void#> .
@prefix terms: <http://purl.org/dc/terms/> .
@prefix schema: <https://schema.org/> .
@prefix dcterms: <http://purl.org/dc/terms> .
@prefix dqv: <http://www.w3.org/ns/dqv#> .
@prefix oa: <http://www.w3.org/ns/oa#> .
@prefix : <http://stream-ontology.com/metrics-severity/> .

<http://stream-ontology.com/metrics-severity/> rdf:type owl:Ontology ;
                             terms:contributor "Norman Radtge"@en ;
                             terms:created "2022-03-15" ;
                             terms:creator "Kurt Junghanns"@en ;
                             terms:title "Metrics severity vocabulary"@en ;
                             <http://purl.org/vocab/vann/preferredNamespacePrefix> "msv" ;
                             <http://purl.org/vocab/vann/preferredNamespaceUri> "http://stream-ontology.com/metrics-severity/" ;
                             rdfs:comment "Vocabulary which extends the Data Quality Vocabulary with a framework to express and calculate the severity of metrics."@en ;
                             rdfs:label "msv: Metrics severity vocabulary"@en ;
                             owl:versionInfo 0.1 ;
                             <https://creativecommons.org/ns#license> "https://creativecommons.org/licenses/by/4.0/" .


#################################################################
#    Object Properties
#################################################################

:hasMaturityLevel a owl:ObjectProperty ;
  rdfs:label "has maturity level"@en ;
  rdfs:comment "The measured maturity level."@en ;
  rdfs:domain dcat:Dataset ;
  rdfs:range :MaturityLevel .

#################################################################
#    Datatype properties
#################################################################

:hasRatingValueOf a owl:DatatypeProperty ;
  rdfs:label "has rating value of"@en ;
  rdfs:comment "A higher number means a higher rating and thus has more weight in calculation of a dqv:Dimensions degree of fulfullment."@en ;
  rdfs:domain dqv:Metric .

:hasMaximumRatingValueOf a owl:DatatypeProperty ;
  rdfs:label "has maximum rating value of"@en ;
  rdfs:comment "The maximum number of corresponding ratings when they are at maximum."@en ;
  rdfs:domain dqv:Dimension .

:hasMinimumRequiredRatingOf a owl:DatatypeProperty ;
  rdfs:label "has minimum required rating of"@en ;
  rdfs:comment "The minimum overall rating this dimension should have."@en ;
  rdfs:domain dqv:Dimension .

:hasRequiredRatingOf a owl:DatatypeProperty ;
  rdfs:label "has required rating of"@en ;
  rdfs:comment "The minimum overall rating this dimension should have."@en ;
  rdfs:domain :MaturityLevel .

:level a owl:DatatypeProperty ;
  rdfs:label "level"@en ;
  rdfs:comment "The level of maturity as a number."@en ;
  rdfs:domain :MaturityLevel .



#################################################################
#    Classes
#################################################################

:MaturityLevel a dqv:QualityCertificate ;
  rdfs:label "Maturity level"@en .

#################################################################
#    Instances
#################################################################

:Motivation a oa:Motivation ;
  rdfs:label "Motivation to execute a dataset quality measurement pipeline" ;
  rdfs:comment "Motivation to execute a dataset quality measurement pipeline using a maturity model and creating a report in HTML." .

:MaturityLevel0 a :MaturityLevel ;
  :hasRequiredRatingOf 0 ;
  :level 0 ;
  oa:hasTarget <http://example.de/dataset1> ; # has to be changed when another dataset is valdiated
  oa:motivatedBy :Motivation ;
  oa:hasBody mme:QMD1 ; # has to be changed on each testset execution
  rdfs:label "Maturity level 0"@en ;
  dc:description "The maturity level which has no requirements and thus applies to every dataset."@en .

:MaturityLevel1 a :MaturityLevel ;
  :hasRequiredRatingOf 32 ;
  :level 1 ;
  oa:hasTarget <http://example.de/dataset1> ; # has to be changed when another dataset is valdiated
  oa:motivatedBy :Motivation ;
  oa:hasBody mme:QMD1 ; # has to be changed on each testset execution
  rdfs:label "Maturity level 1"@en ;
  dc:description "The maturity level which has the highest requirements in which all dimensions have to have the maximum rating value."@en .
